\documentclass[12pt]{article}
\usepackage{amsmath}
\begin{document}
\title{Chapter 1: Matrix Operations \\ Section 5: Cramer's Rule}
\author{Alec Mouri}

\maketitle
\section*{Exercises}
\begin{itemize}
\item[(1)]
$$A^{-1} = \frac{1}{ad - bc}\begin{bmatrix}
d & -b \\
-c & d
\end{bmatrix} = \begin{bmatrix}
d & -b \\
-c & d
\end{bmatrix}$$
\item[(2)]
$$\text{adj }\begin{bmatrix}
1 & 2 \\
3 & 4
\end{bmatrix} = \begin{bmatrix}
4 & -2 \\
-3 & 1
\end{bmatrix}$$
$$\det\begin{bmatrix}
1 & 2 \\
3 & 4
\end{bmatrix} = (1)(4) - (2)(3) = -2$$
$$\begin{bmatrix}
4 & -2 \\
-3 & 1
\end{bmatrix}\begin{bmatrix}
1 & 2 \\
3 & 4
\end{bmatrix} = \begin{bmatrix}
-2 & 0 \\
0 & -2
\end{bmatrix}$$
$$\begin{bmatrix}
1 & 2 \\
3 & 4
\end{bmatrix}\begin{bmatrix}
4 & -2 \\
-3 & 1
\end{bmatrix} = \begin{bmatrix}
-2 & 0 \\
0 & -2
\end{bmatrix}$$
$$\text{adj }\begin{bmatrix}
1 & 1 & 2 \\
2 & 4 & 2 \\
0 & 2 & 1
\end{bmatrix} = \begin{bmatrix}
\det\begin{bmatrix}
4 & 2 \\
2 & 1
\end{bmatrix} & - \det\begin{bmatrix}
1 & 2 \\
2 & 1
\end{bmatrix} & \det\begin{bmatrix}
1 & 2 \\
4 & 2
\end{bmatrix} \\
-\det\begin{bmatrix}
2 & 2 \\
0 & 1
\end{bmatrix} & \det\begin{bmatrix}
1 & 2 \\
0 & 1
\end{bmatrix} & -\det\begin{bmatrix}
1 & 2 \\
2 & 2
\end{bmatrix} \\
\det\begin{bmatrix}
2 & 4 \\
0 & 2
\end{bmatrix} & -\det\begin{bmatrix}
1 & 1 \\
0 & 2
\end{bmatrix} & \det\begin{bmatrix}
1 & 1 \\
2 & 4
\end{bmatrix}
\end{bmatrix}$$
$$= \begin{bmatrix}
0 & 3 & -6 \\
-2 & 1 & 2 \\
4 & -2 & 2
\end{bmatrix}$$
$$\det\begin{bmatrix}
1 & 1 & 2 \\
2 & 4 & 2 \\
0 & 2 & 1
\end{bmatrix} = 1(4 - 4) - 2(1 - 4) = 6$$
$$\begin{bmatrix}
1 & 1 & 2 \\
2 & 4 & 2 \\
0 & 2 & 1
\end{bmatrix}\begin{bmatrix}
0 & 3 & -6 \\
-2 & 1 & 2 \\
4 & -2 & 2
\end{bmatrix} = \begin{bmatrix}
6 & 0 & 0 \\
0 & 6 & 0 \\
0 & 0 & 6
\end{bmatrix}$$
$$\begin{bmatrix}
0 & 3 & -6 \\
-2 & 1 & 2 \\
4 & -2 & 2
\end{bmatrix}\begin{bmatrix}
1 & 1 & 2 \\
2 & 4 & 2 \\
0 & 2 & 1
\end{bmatrix} = \begin{bmatrix}
6 & 0 & 0 \\
0 & 6 & 0 \\
0 & 0 & 6
\end{bmatrix}$$
$$\text{adj }\begin{bmatrix}
4 & -1 & 1 \\
1 & 1 & -2 \\
1 & -1 & 1
\end{bmatrix}$$
$$= \begin{bmatrix}
\det\begin{bmatrix}
1 & -2 \\
-1 & 1
\end{bmatrix} & -\det\begin{bmatrix}
-1 & 1 \\
-1 & 1
\end{bmatrix} & \det\begin{bmatrix}
-1 & 1 \\
1 & -2
\end{bmatrix} \\
-\det\begin{bmatrix}
1 & -2 \\
1 & 1
\end{bmatrix} & \det\begin{bmatrix}
4 & 1 \\
1 & 1
\end{bmatrix} & -\det\begin{bmatrix}
4 & 1 \\
1 & -2
\end{bmatrix} \\
\det\begin{bmatrix}
1 & 1 \\
1 & -1
\end{bmatrix} & -\det\begin{bmatrix}
4 & -1 \\
1 & -1
\end{bmatrix} & \det\begin{bmatrix}
4 & -1 \\
1 & 1
\end{bmatrix}
\end{bmatrix}$$
$$= \begin{bmatrix}
-1 & 0 & 1 \\
-3 & 3 & 9 \\
-2 & 3 & 5
\end{bmatrix}$$
$$\det\begin{bmatrix}
4 & -1 & 1 \\
1 & 1 & -2 \\
1 & -1 & 1
\end{bmatrix} = 4\det\begin{bmatrix}
1 & -2 \\
-1 & 1
\end{bmatrix} - \det\begin{bmatrix}
-1 & 1 \\
-1 & 1
\end{bmatrix} + \det\begin{bmatrix}
-1 & 1 \\
1 & -2
\end{bmatrix} $$
$$= 4(1 - 2) - (-1 + 1) + (2 - 1) = -3$$
$$\begin{bmatrix}
4 & -1 & 1 \\
1 & 1 & -2 \\
1 & -1 & 1
\end{bmatrix}\begin{bmatrix}
-1 & 0 & 1 \\
-3 & 3 & 9 \\
-2 & 3 & 5
\end{bmatrix} = \begin{bmatrix}
-3 & 0 & 0 \\
0 & -3 & 0 \\
0 & 0 & -3
\end{bmatrix}$$
$$\begin{bmatrix}
-1 & 0 & 1 \\
-3 & 3 & 9 \\
-2 & 3 & 5
\end{bmatrix}\begin{bmatrix}
4 & -1 & 1 \\
1 & 1 & -2 \\
1 & -1 & 1
\end{bmatrix} = \begin{bmatrix}
-3 & 0 & 0 \\
0 & -3 & 0 \\
0 & 0 & -3
\end{bmatrix}$$
$$\text{adj }\begin{bmatrix}
a & b & c \\
1 & 0 & 1 \\
1 & 1 & 1
\end{bmatrix} = \begin{bmatrix}
\det\begin{bmatrix}
0 & 1 \\
1 & 1
\end{bmatrix} & -\det\begin{bmatrix}
b & c \\
1 & 1
\end{bmatrix} & \det\begin{bmatrix}
b & c \\
0 & 1
\end{bmatrix} \\
-\det\begin{bmatrix}
1 & 1 \\
1 & 1
\end{bmatrix} & \det\begin{bmatrix}
a & c \\
1 & 1
\end{bmatrix} & -\det\begin{bmatrix}
a & c \\
1 & 1
\end{bmatrix} \\
\det\begin{bmatrix}
1 & 0 \\
1 & 1
\end{bmatrix} & -\det\begin{bmatrix}
a & b \\
1 & 1
\end{bmatrix} & \det\begin{bmatrix}
a & b \\
1 & 0
\end{bmatrix}
\end{bmatrix}$$
$$= \begin{bmatrix}
-1 & c - b & b \\
0 & a - c & c - a \\
1 & b - a & -b
\end{bmatrix}$$
$$\det\begin{bmatrix}
a & b & c \\
1 & 0 & 1 \\
1 & 1 & 1
\end{bmatrix} = a\begin{bmatrix}
0 & 1 \\
1 & 1
\end{bmatrix} - \begin{bmatrix}
b & c \\
1 & 1
\end{bmatrix} + \begin{bmatrix}
b & c \\
0 & 1
\end{bmatrix}$$
$$= a(0 - 1) - (b - c) + (b - 0) = c - a$$
$$\begin{bmatrix}
a & b & c \\
1 & 0 & 1 \\
1 & 1 & 1
\end{bmatrix}\begin{bmatrix}
-1 & c - b & b \\
0 & a - c & c - a \\
1 & b - a & -b
\end{bmatrix}$$
$$= \begin{bmatrix}
c - a & ac - ab + ab - bc + bc - ac & ab + bc  - ab - bc \\
-1 + 1 & c - b + b - a & b - b \\
-1 + 1 & c - b + a - c + b - a & b + c - a - b
\end{bmatrix} $$
$$= \begin{bmatrix}
c - a & 0 & 0 \\
0 & c - a & 0 \\
0 & 0 & c - a
\end{bmatrix}$$
$$\begin{bmatrix}
-1 & c - b & b \\
0 & a - c & c - a \\
1 & b - a & -b
\end{bmatrix}\begin{bmatrix}
a & b & c \\
1 & 0 & 1 \\
1 & 1 & 1
\end{bmatrix}$$
$$= \begin{bmatrix}
-a + c - b + b & -b + b & -c + c - b + b \\
a - c + c - a & c - a & a - c + c - a \\
a + b - a - b & b - b & c + b - a - b
\end{bmatrix} = \begin{bmatrix}
c - a & 0 & 0 \\
0 & c - a & 0 \\
0 & 0 & c - a
\end{bmatrix}$$
\item[(3)]
Suppose $A^{-1}$ has integer entries. we have that
$$\det(A^{-1}A) = \det I = 1$$
and
$$\det(A^{-1}A) = \det A^{-1}\det A$$
Since $A$ has integer entries, then $\det A$ and $\det A^{-1}$ are also integers. So, we have $\det A = \frac{1}{\det A^{-1}}$, and therefore $\det A^{-1} = \pm 1$.

Suppose $\det A = \pm 1$. Then $A^{-1} = \frac{1}{\det A}\text{adj }A = \pm \text{adj }A$. Since $\pm\text{adj}_{ij} = \pm(-1)^{ij}\det A_{ji}$ is composed from the multiplication and addition of integers, then $\pm \text{adj A}$ has entirely integer entries. Therefore, $A^{-1}$ has entirely integer entries.
\item[(4)]
$$\det A = \det A^\top = \sum_{i=1}^n a_{1i}\det A_{1i}^\top = \sum_{i=1}^n a_{1i}\det A_{1i}$$
\end{itemize}
\end{document}